spectec/src/backend-interpreter/interpreter.mli
@@ -1,4 +1,5 @@
 open Al.Ast
 
+val builtin_hint_id: string
 val instantiate: value list -> value
 val invoke: value list -> value
