spectec/test-lean-backend/potential_bug_scraps/bug_example.lean
@@ -1,0 +1,27 @@
+def List.ap (fs : List (α → β)) (xs : List α) : List β :=
+  List.zipWith ((· ·)) fs xs
+
+def Option.ap (f : Option (α → β)) (x : Option α) : Option β :=
+  f.bind (fun f => x.map f)
+
+opaque rat_to_nat (r : Rat) : Nat := by
+  first
+     | exact Inhabited.default
+     | intros ; assumption
+
+
+/- Inductive Type Definition at: test-lean-backend/potential_bug_scraps/bug_example.spectec:10.1-10.21 -/
+inductive marker : Type where
+  | MARK : marker
+deriving Inhabited, BEq, DecidableEq, ReflBEq, LawfulBEq
+
+/- Inductive Type Definition at: test-lean-backend/potential_bug_scraps/bug_example.spectec:12.1-13.20 -/
+inductive thing : Type where
+  | THING (marker_opt : Option marker) (_ : Nat) : thing
+deriving Inhabited, BEq, DecidableEq, ReflBEq, LawfulBEq
+
+/- Inductive Relations Definition at: test-lean-backend/potential_bug_scraps/bug_example.spectec:17.1-17.30 -/
+inductive Thing_ok : thing → Prop where
+  | mk_Thing_ok (n : Nat) :
+    n > 0 →
+    Thing_ok (thing.THING (some marker.MARK) n)
