spectec/test-lean-backend/potential_bug_scraps/legitimate_example.lean
@@ -1,0 +1,28 @@
+def List.ap (fs : List (α → β)) (xs : List α) : List β :=
+  List.zipWith ((· ·)) fs xs
+
+def Option.ap (f : Option (α → β)) (x : Option α) : Option β :=
+  f.bind (fun f => x.map f)
+
+opaque rat_to_nat (r : Rat) : Nat := by
+  first
+     | exact Inhabited.default
+     | intros ; assumption
+
+
+/- Inductive Type Definition at: test-lean-backend/potential_bug_scraps/legitimate_example.spectec:7.1-7.25 -/
+inductive tag : Type where
+  | SMALL : tag
+  | BIG : tag
+deriving Inhabited, BEq, DecidableEq, ReflBEq, LawfulBEq
+
+/- Inductive Type Definition at: test-lean-backend/potential_bug_scraps/legitimate_example.spectec:9.1-9.18 -/
+inductive marker : Type where
+  | X : marker
+deriving Inhabited, BEq, DecidableEq, ReflBEq, LawfulBEq
+
+/- Auxiliary Definition at: test-lean-backend/potential_bug_scraps/legitimate_example.spectec:11.1-11.26 -/
+def extra (v_tag : tag) : Option marker :=
+  match v_tag with
+  | tag.SMALL => none
+  | tag.BIG => some marker.X
