spectec/test-lean/family-hint-repro/toy.lean
@@ -1,0 +1,94 @@
+def List.ap (fs : List (α → β)) (xs : List α) : List β :=
+  List.zipWith ((· ·)) fs xs
+
+def Option.ap (f : Option (α → β)) (x : Option α) : Option β :=
+  f.bind (fun f => x.map f)
+
+opaque rat_to_nat (r : Rat) : Nat := by
+  first
+     | exact Inhabited.default
+     | intros ; assumption
+
+
+/- Inductive Type Definition at: test-lean/family-hint-repro/toy.spectec:5.1-5.39 -/
+inductive numtype : Type where
+  | I32 : numtype
+  | I64 : numtype
+  | F32 : numtype
+  | F64 : numtype
+deriving Inhabited, BEq, DecidableEq, ReflBEq, LawfulBEq
+
+/- Inductive Type Definition at: test-lean/family-hint-repro/toy.spectec:6.1-6.22 -/
+inductive vectype : Type where
+  | V128 : vectype
+deriving Inhabited, BEq, DecidableEq, ReflBEq, LawfulBEq
+
+/- Inductive Type Definition at: test-lean/family-hint-repro/toy.spectec:8.1-8.23 -/
+inductive Inn : Type where
+  | I32 : Inn
+  | I64 : Inn
+deriving Inhabited, BEq, DecidableEq, ReflBEq, LawfulBEq
+
+/- Auxiliary Definition at:  -/
+def numtype_Inn (var_0 : Inn) : numtype :=
+  match var_0 with
+  | Inn.I32 => numtype.I32
+  | Inn.I64 => numtype.I64
+
+/- Inductive Type Definition at: test-lean/family-hint-repro/toy.spectec:9.1-9.23 -/
+inductive Fnn : Type where
+  | F32 : Fnn
+  | F64 : Fnn
+deriving Inhabited, BEq, DecidableEq, ReflBEq, LawfulBEq
+
+/- Auxiliary Definition at:  -/
+def numtype_Fnn (var_0 : Fnn) : numtype :=
+  match var_0 with
+  | Fnn.F32 => numtype.F32
+  | Fnn.F64 => numtype.F64
+
+/- Inductive Type Definition at: test-lean/family-hint-repro/toy.spectec:10.1-10.18 -/
+inductive Vnn : Type where
+  | V128 : Vnn
+deriving Inhabited, BEq, DecidableEq, ReflBEq, LawfulBEq
+
+/- Inductive Type Definition at: test-lean/family-hint-repro/toy.spectec:12.1-12.21 -/
+inductive num_ : Type where
+  | mk_num__0 (v_Inn : Inn) (var_x : Nat) : num_
+  | mk_num__1 (v_Fnn : Fnn) (var_x : Nat) : num_
+deriving Inhabited, BEq, DecidableEq, ReflBEq, LawfulBEq
+
+/- Inductive Relations Definition at: test-lean/family-hint-repro/toy.spectec:12.8-12.13 -/
+inductive wf_num_ : numtype → num_ → Prop where
+  | num__case_0 (v_numtype : numtype) (v_Inn : Inn) (var_x : Nat) :
+    v_numtype = (numtype_Inn v_Inn) →
+    wf_num_ v_numtype (num_.mk_num__0 v_Inn var_x)
+  | num__case_1 (v_numtype : numtype) (v_Fnn : Fnn) (var_x : Nat) :
+    v_numtype = (numtype_Fnn v_Fnn) →
+    wf_num_ v_numtype (num_.mk_num__1 v_Fnn var_x)
+
+
+/- Auxiliary Definition at: test-lean/family-hint-repro/toy.spectec:12.1-12.21 -/
+def proj_num__0 (var_x : num_) : Option Nat :=
+  match var_x with
+  | num_.mk_num__0 v_Inn var_x => some var_x
+  | _ => none
+
+/- Auxiliary Definition at: test-lean/family-hint-repro/toy.spectec:12.1-12.21 -/
+def proj_num__1 (var_x : num_) : Option Nat :=
+  match var_x with
+  | num_.mk_num__1 v_Fnn var_x => some var_x
+  | _ => none
+
+/- Type Alias Definition at: test-lean/family-hint-repro/toy.spectec:16.1-16.27 -/
+abbrev vec_ : Type := Nat
+
+/- Auxiliary Definition at: test-lean/family-hint-repro/toy.spectec:18.1-18.55 -/
+def foo (v_numtype : numtype) (v_num_ : num_) : Option (List Nat) :=
+  none
+
+/- Axiom Definition at: test-lean/family-hint-repro/toy.spectec:19.1-19.55 -/
+opaque bar (v_vectype : vectype) (v_vec_ : vec_) : List Nat := by
+  first
+     | exact Inhabited.default
+     | intros ; assumption
